



Given Polynomial = y_1

$$y_1 = 6L\left(\frac{\theta}{\beta}\right)^2 - 8L\left(\frac{\theta}{\beta}\right)^3 + 3L\left(\frac{\theta}{\beta}\right)^4$$

$$y_1' = 12L\theta/\beta^2 - 24L\theta^2/\beta^3 + 12L\theta^3/\beta^4$$

$$y_1'' = 12L/\beta^2 - 48L\theta/\beta^3 + 36L\theta^2/\beta^4$$

SECTION	EQUATION
1	Given Polynomial
2	Constant
3	Half-Return Cycloidal (a)
4	Linear
5	Half-Return Harmonic (b)

$$L_1 = 6.7 \text{ in} \quad \beta_1 = 2.677 \text{ rad}$$

$$L_2 = 0 \text{ in} \quad \beta_2 = 20^\circ = 0.349 \text{ rad}$$

$$L_3 = 4.43 \text{ in} \quad \beta_3 = 2.446 \text{ rad}$$

$$L_4 = 1.1 \text{ in} \quad \beta_4 = 0.304 \text{ rad}$$

$$L_5 = 1.17 \text{ in} \quad \beta_5 = 0.507 \text{ rad}$$

$$\omega = 58 \text{ rpm} = 6.07 \text{ rad/s}$$

$$\dot{y}_4 = -22 \text{ in/s}$$

$$y_4' = \dot{y}_4/\omega = -4.116 \text{ in/rad} = m$$

$$\beta_4 = L_4/y_4' = 0.2672 \text{ rad}$$

$$\textcircled{1} \quad y_3'\left(\frac{\theta}{\beta} = 1\right) = m$$

$$\textcircled{2} \quad y_5'\left(\frac{\theta}{\beta} = 0\right) = m$$

$$\textcircled{3} \quad y_5''\left(\frac{\theta}{\beta} = 1\right) = y_1''\left(\frac{\theta}{\beta} = 0\right)$$

$$\textcircled{4} \quad L_3 + L_4 + L_5 = L_1$$

$$\textcircled{5} \quad \beta_1 + \beta_2 + \beta_3 + \beta_4 + \beta_5 = 2\pi \text{ rad}$$